freshly generated pts

theories/SemiUnification/autosubst/pts.sig
@@ -1,0 +1,7 @@
+nat : Type
+term : Type
+
+const : nat -> term
+app : term -> term -> term
+lam : term -> (term -> term) -> term
+Pi : term -> (term -> term) -> term
