theories/SemiUnification/autosubst/pts_more.v
@@ -2,6 +2,7 @@
 Here, I use ssreflect for convenience. Actual generated proofs should be terms.
 *)
 
+Require Import Undecidability.SemiUnification.autosubst.unscoped.
 Require Import Undecidability.SemiUnification.autosubst.pts.
 Require Import Undecidability.SemiUnification.autosubst.unscoped_more.
 
@@ -73,3 +74,176 @@ Definition term_norm := (compRen_term, renRen_term, @ren_term_id, renComp_term, 
 Arguments funcomp {X Y Z} _ _ _ /.
 (* such that simpl evaluates id x*)
 Arguments unscoped.id _ _/.
+
+(* AUTOSUBST EXPERIMENTS *)
+
+Lemma ad {X Y: Type} {s: X} {f: nat -> Y} {g: Y -> X} {t: Y}: 
+  s = g t ->
+  forall x, scons s (funcomp g f) x = funcomp g (scons t f) x.
+Proof.
+  move=> H. by case.
+Qed.
+
+(* this is the important property! not ad-hoc, no sigma*)
+Definition up_subst_ren_term_term_underlying
+(zeta_term : forall _ : nat, nat): forall s,
+ren_term (upRen_term_term zeta_term) (ren_term ↑ s) =
+ren_term ↑ (ren_term zeta_term s) :=
+fun (s : term) =>
+  eq_trans
+    (compRenRen_term ↑ (upRen_term_term zeta_term) 
+    (zeta_term >> ↑) (fun x : nat => eq_refl) s)
+    (eq_sym
+      (compRenRen_term zeta_term ↑ (zeta_term >> ↑) 
+          (fun x : nat => eq_refl) s)).
+
+(* this is the important property! not ad-hoc, no sigma*)
+Definition up_subst_subst_term_term_underlying
+(tau_term : forall _ : nat, term): forall s,
+subst_term (up_term_term tau_term) (ren_term shift s) =
+ren_term shift (subst_term tau_term s) :=
+fun (s : term) =>
+eq_trans
+  (compRenSubst_term ↑ (up_term_term tau_term) (tau_term >> ren_term ↑)
+   (fun _ => eq_refl) s)
+  (eq_sym
+     (compSubstRen_term tau_term ↑ (tau_term >> ren_term ↑)
+        (fun _ => eq_refl) s)).
+
+(*
+H is ren_term shift
+z is var 0
+
+F f : subst_term f
+G f : subst_term (up_term_term f)
+
+or
+
+F f : ren_term f
+G f : ren_term (upRen_term_term f)
+*)
+
+(* maybe this is even more general ? *)
+(* does not depend on term *)
+Definition more_general_principle3 {X Y : Type}
+  {sigma : nat -> Y} {F: (nat -> X) -> Y -> Y} {G: X -> X} {H: Y -> Y}
+  {tau_term : nat -> X} {theta : nat -> Y} {x: X} (y: Y)
+  (Eq : forall x, funcomp (F tau_term) sigma x = theta x)
+  (Eq1 : F (x .: tau_term >> G) y = y)
+  (Eq2 : forall s, F (x .: tau_term >> G) (H s) = F (tau_term >> G) s)
+  (Eq3 : forall s, H (F tau_term s) = F (tau_term >> G) s)
+  :
+  forall (n: nat),
+  (funcomp (F (x .: tau_term >> G)) (scons y (sigma >> H)) n) = 
+  (scons y (theta >> H) n).
+Proof.
+  intros [|n].
+  - apply Eq1.
+  - apply (eq_trans (Eq2 _)).
+    apply (eq_trans (eq_sym (Eq3 _))).
+    apply (ap H).
+    apply Eq.
+Qed.
+
+(*showcase 1 more_general_principle3 *)
+Definition up_subst_subst_term_term_using_test (sigma : forall _ : nat, term)
+  (tau_term : forall _ : nat, term) (theta : forall _ : nat, term)
+  (Eq : forall x, eq (funcomp (subst_term tau_term) sigma x) (theta x)) :
+  forall x,
+  eq (funcomp (subst_term (up_term_term tau_term)) (up_term_term sigma) x)
+    (up_term_term theta x).
+Proof.
+  eapply (more_general_principle3).
+  exact Eq.
+  reflexivity.
+  apply compRenSubst_term.
+  reflexivity.
+  apply compSubstRen_term.
+  reflexivity.
+  Show Proof.
+Qed.
+
+(*showcase 2 more_general_principle3 *)
+Definition up_subst_ren_term_term (sigma : forall _ : nat, term)
+         (zeta_term : forall _ : nat, nat) (theta : forall _ : nat, term)
+         (Eq : forall x, eq (funcomp (ren_term zeta_term) sigma x) (theta x)) :
+         forall x,
+         eq (funcomp (ren_term (upRen_term_term zeta_term)) (up_term_term sigma) x)
+           (up_term_term theta x).
+Proof.
+  eapply (more_general_principle3).
+  exact Eq.
+  reflexivity.
+  apply compRenRen_term.
+  reflexivity.
+  apply compRenRen_term.
+  reflexivity.
+  Show Proof.
+Qed.
+
+
+(* this is maybe the general lemma 
+independent of autosubst (unscoped)
+skeleton of the actual proof *)
+Definition more_general_principle2 {X Y : Type}
+  (sigma : nat -> Y) {F G: X -> Y -> Y} {H: Y -> Y}
+  (tau_term : X) (theta : nat -> Y) (z: Y)
+  (Eq : forall x, funcomp (F tau_term) sigma x = theta x)
+  (Eq1 : G tau_term z = z)
+  (Eq2 : forall s, G tau_term (H s) = H (F tau_term s))
+  :
+  forall (x: nat),
+  (funcomp (G tau_term) (scons z (sigma >> H)) x) = 
+  (scons z (theta >> H) x).
+Proof.
+  intros [|x].
+  - apply Eq1.
+  - eapply eq_trans.
+    apply Eq2.
+    apply (ap H). apply Eq.
+    Show Proof.
+Qed.
+
+(*showcase 1 more_general_principle2 *)
+Definition up_subst_subst_term_term_using_test' (sigma : forall _ : nat, term)
+  (tau_term : forall _ : nat, term) (theta : forall _ : nat, term)
+  (Eq : forall x, eq (funcomp (subst_term tau_term) sigma x) (theta x)) :
+  forall x,
+  eq (funcomp (subst_term (up_term_term tau_term)) (up_term_term sigma) x)
+    (up_term_term theta x).
+Proof.
+  eapply (more_general_principle2 _ _ (G := (fun tau_term => subst_term (up_term_term tau_term)))). 
+  exact Eq.
+  reflexivity.
+  apply up_subst_subst_term_term_underlying.
+  Show Proof.
+Qed.
+
+(*showcase 2 more_general_principle2 *)
+Definition up_subst_ren_term_term' (sigma : forall _ : nat, term)
+         (zeta_term : forall _ : nat, nat) (theta : forall _ : nat, term)
+         (Eq : forall x, eq (funcomp (ren_term zeta_term) sigma x) (theta x)) :
+         forall x,
+         eq (funcomp (ren_term (upRen_term_term zeta_term)) (up_term_term sigma) x)
+           (up_term_term theta x).
+Proof.
+  eapply (more_general_principle2 _ _ (G := (fun zeta_term => ren_term (upRen_term_term zeta_term)))).
+  exact Eq.
+  reflexivity.
+  apply up_subst_ren_term_term_underlying.
+  Show Proof.
+Qed.
+           
+
+Definition up_subst_subst_term_term (sigma : forall _ : nat, term)
+  (tau_term : forall _ : nat, term) (theta : forall _ : nat, term)
+  (Eq : forall x, eq (funcomp (subst_term tau_term) sigma x) (theta x)) :
+  forall x,
+  eq (funcomp (subst_term (up_term_term tau_term)) (up_term_term sigma) x)
+    (up_term_term theta x) :=
+  fun x => match x with
+    | 0 => eq_refl
+    | S x' =>
+        eq_trans (up_subst_subst_term_term_underlying tau_term (sigma x'))
+          (ap (ren_term ↑) (Eq x'))
+    end.
